theories/GraphCore/TensorGraphQuote.v
@@ -1,0 +1,806 @@
+Require Export TensorGraphHom.
+
+(* TODO: Quote from CospanHyperGraph T to
+  CospanHyperGraph positive, via CospanHyperGraph (option T).
+  Prove can test for isomorphism in quoted. *)
+
+(* FIXME: Move *)
+Lemma graph_of_tensor_cohg_eq `{Equiv T} (t t' : T) n m : t ≡ t' ->
+  cohg_eq (graph_of_tensor t n m) (graph_of_tensor t' n m).
+Proof.
+  intros Ht.
+  apply mk_cohg_eq; [done..|].
+  cbn.
+  split; [|done].
+  rewrite 2 hyperedges_singleton.
+  rewrite <- insert_empty.
+  apply insert_proper; [|apply map_empty_equiv_eq; done].
+  split; [split;[|done]|done].
+  apply Ht.
+Qed.
+
+Add Parametric Morphism `{Equiv T, Equivalence T equiv}
+  {n m o} : (@compose_graphs_aux T n m o)
+  with signature cohg_eq ==> cohg_eq ==> cohg_eq
+  as compose_graphs_aux_cohg_eq.
+Proof.
+  intros cohg1 cohg1' (Hin1 & Hout1 & He1)
+    cohg2 cohg2' (Hin2 & Hout2 & He2).
+  unfold compose_graphs_aux.
+  rewrite <- Hin1, <- Hout1, <- Hin2, <- Hout2.
+  f_equiv.
+  apply mk_cohg_eq; [done..|].
+  cbn.
+  now do 2 f_equiv.
+Qed.
+
+Add Parametric Morphism `{Equiv T, Equivalence T equiv}
+  {n m o} : (@compose_graphs T n m o)
+  with signature cohg_eq ==> cohg_eq ==> cohg_eq
+  as compose_graphs_cohg_eq.
+Proof.
+  intros cohg1 cohg1' Heq1
+    cohg2 cohg2' Heq2.
+  rewrite 2 compose_graphs_to_compose_graphs_aux.
+  now do 3 f_equiv.
+Qed.
+
+Add Parametric Morphism `{Equiv T, Equivalence T equiv}
+  {n m o} : (@compose_graphs_unsafe T n m o)
+  with signature cohg_eq ==> cohg_eq ==> cohg_eq
+  as compose_graphs_unsafe_cohg_eq.
+Proof.
+  intros cohg1 cohg1' (Hin1 & Hout1 & He1)
+    cohg2 cohg2' (Hin2 & Hout2 & He2).
+  unfold compose_graphs_unsafe.
+  rewrite <- Hin1, <- Hin2, <- Hout2.
+  apply mk_cohg_eq; [done..|].
+  cbn.
+  now do 2 f_equiv.
+Qed.
+
+Add Parametric Morphism `{Equiv T} {n m} : (@referrenced_vertices T n m)
+  with signature cohg_eq ==> eq as referrenced_vertices_cohg_eq.
+Proof.
+  intros cohg cohg' (Hins & Houts & [Heq Hverts]).
+  unfold referrenced_vertices.
+  rewrite <- Hins, Houts.
+  f_equal.
+  apply map_to_list_equiv in Heq.
+  induction Heq as [|? ? ? ? Hhd]; [done|].
+  cbn.
+  rewrite 2 (list_to_set_app_L (_++_)).
+  f_equal; [|done].
+  do 2 f_equal; apply Hhd.
+Qed.
+
+Add Parametric Morphism `{Equiv T} {n m} : (@isolated_vertices T n m)
+  with signature cohg_eq ==> eq as isolated_vertices_cohg_eq.
+Proof.
+  intros cohg cohg' Heq.
+  unfold isolated_vertices.
+  f_equal; [|now rewrite Heq].
+  apply Heq.2.2.2.
+Qed.
+
+Add Parametric Morphism `{Equiv T} {n m} : (@set_verts T n m)
+  with signature cohg_eq ==> eq ==> cohg_eq as set_verts_cohg_eq.
+Proof.
+  intros cohg cohg' (Hins & Houts & [Heq Hverts]) vs.
+  apply mk_cohg_eq; [done..|].
+  split; [done|].
+  done.
+Qed.
+
+
+Add Parametric Morphism `{Equiv T} {n m} : (@norm_verts T n m)
+  with signature cohg_eq ==> cohg_eq as norm_verts_cohg_eq.
+Proof.
+  intros cohg cohg' Heq.
+  unfold norm_verts.
+  now apply set_verts_cohg_eq, isolated_vertices_cohg_eq_Proper.
+Qed.
+
+
+
+
+
+
+
+
+Class CospanHyperGraphQuote {Ctx T} `{Equiv T'} (f : Ctx -> T -> T')
+  (ctx : Ctx) {n m} (expr : CospanHyperGraph T n m) (val : CospanHyperGraph T' n m) := {
+  cohg_quote : cohg_eq (graph_apply_hom (f ctx) expr) val;
+}.
+
+#[global] Hint Mode CospanHyperGraphQuote + + + - + - + + - + : typeclass_instances.
+
+Class AbstractTensorQuote {Ctx T} `{Equiv T'} (f : Ctx -> T -> T') (ctx : Ctx)
+  (t : T) (t' : T') := {
+  abs_quote : f ctx t ≡ t'
+}.
+
+#[global] Hint Mode AbstractTensorQuote + + + - + + - + : typeclass_instances.
+
+
+Lemma cohg_quote_correct_equiv {Ctx} `{Equiv T, Equivalence T equiv,
+  Equiv T', Equivalence T' equiv}
+  (f : Ctx -> T -> T')
+  (ctx : Ctx) {n m} (expr expr' : CospanHyperGraph T n m)
+    (val val' : CospanHyperGraph T' n m)
+    {Hval : CospanHyperGraphQuote f ctx expr val}
+    {Hval' : CospanHyperGraphQuote f ctx expr' val'}
+    {Hf : Proper (equiv ==> equiv) (f ctx)} :
+  expr ≡ expr' -> val ≡ val'.
+Proof.
+  intros Heq.
+  destruct Hval as [Hval].
+  destruct Hval' as [Hval'].
+  rewrite <- Hval.
+  etransitivity; [|apply cohg_eq_subrelation, Hval'].
+  refine (graph_apply_hom_proper_Proper _ _ _ _ _).
+  done.
+Qed.
+
+
+Section instances.
+
+#[local] Set Typeclasses Unique Instances.
+
+Context {Ctx T} `{Equiv T'} `{Equivalence T' equiv} (f : Ctx -> T -> T')
+  (ctx : Ctx).
+
+Local Notation Quote := (@CospanHyperGraphQuote Ctx T T' _ f ctx _ _).
+
+#[export] Instance cohg_quote_graph_apply_hom {n m} (expr : CospanHyperGraph T n m) :
+  Quote expr (graph_apply_hom (f ctx) expr).
+Proof.
+  now constructor.
+Qed.
+
+#[export] Instance cohg_quote_id_graph {n} : Quote (id_graph n) (id_graph n).
+Proof.
+  constructor.
+  done.
+Qed.
+
+#[export] Instance cohg_quote_cup_graph {n} : Quote (cup_graph n) (cup_graph n).
+Proof.
+  constructor.
+  done.
+Qed.
+
+#[export] Instance cohg_quote_cap_graph {n} : Quote (cap_graph n) (cap_graph n).
+Proof.
+  constructor.
+  done.
+Qed.
+
+#[export] Instance cohg_quote_swap_graph {n m} : Quote (swap_graph n m) (swap_graph n m).
+Proof.
+  constructor.
+  done.
+Qed.
+
+#[export] Instance cohg_quote_graph_of_tensor {n m} t t' :
+  AbstractTensorQuote f ctx t t' ->
+  Quote (graph_of_tensor t n m) (graph_of_tensor t' n m).
+Proof.
+  intros [Ht].
+  constructor.
+  rewrite graph_apply_hom_graph_of_tensor.
+  now apply graph_of_tensor_cohg_eq.
+Qed.
+
+Lemma quote_of_unary_mor {n m n' m'}
+  (g : forall T'', CospanHyperGraph T'' n m -> CospanHyperGraph T'' n' m')
+  (Hg : Proper (cohg_eq ==> cohg_eq) (g T'))
+  (Hghom : forall cohg, graph_apply_hom (f ctx) (g T cohg) =
+      g T' (graph_apply_hom (f ctx) cohg)) :
+  forall expr val, Quote expr val -> Quote (g T expr) (g T' val).
+Proof.
+  intros expr val [Hval].
+  constructor.
+  rewrite Hghom.
+  now apply Hg.
+Qed.
+
+Lemma quote_of_binary_mor {n m n' m' n'' m''}
+  (g : forall T'', CospanHyperGraph T'' n m -> CospanHyperGraph T'' n' m' ->
+    CospanHyperGraph T'' n'' m'')
+  (Hg : Proper (cohg_eq ==> cohg_eq ==> cohg_eq) (g T'))
+  (Hghom : forall cohg cohg', graph_apply_hom (f ctx) (g T cohg cohg') =
+      g T' (graph_apply_hom (f ctx) cohg) (graph_apply_hom (f ctx) cohg')) :
+  forall expr expr' val val', Quote expr val -> Quote expr' val' ->
+    Quote (g T expr expr') (g T' val val').
+Proof.
+  intros expr expr' val val' [Hval] [Hval'].
+  constructor.
+  rewrite Hghom.
+  now apply Hg.
+Qed.
+
+#[export] Instance cohg_quote_relabel_graph {n m}
+  g (expr : CospanHyperGraph T n m) val :
+  Quote expr val ->
+  Quote (relabel_graph g expr)
+    (relabel_graph g val).
+Proof.
+  apply (quote_of_unary_mor (fun _ => _) _).
+  intros; apply graph_apply_hom_relabel_graph.
+Qed.
+
+#[export] Instance cohg_quote_reindex_graph {n m}
+  g (expr : CospanHyperGraph T n m) val :
+  Quote expr val ->
+  Quote (reindex_graph g expr)
+    (reindex_graph g val).
+Proof.
+  apply (quote_of_unary_mor (fun _ => _) _).
+  intros; apply graph_apply_hom_reindex_graph.
+Qed.
+
+#[export] Instance cohg_quote_swapped_stack_graphs_aux {n m n' m'}
+  (expr : CospanHyperGraph T n m) (expr' : CospanHyperGraph T n' m')
+  val val' :
+  Quote expr val -> Quote expr' val' ->
+  Quote (swapped_stack_graphs_aux expr expr')
+    (swapped_stack_graphs_aux val val').
+Proof.
+  apply (quote_of_binary_mor (fun _ => _) _).
+  intros; apply graph_apply_hom_swapped_stack_graphs_aux.
+Qed.
+
+#[export] Instance cohg_quote_swapped_stack_graphs {n m n' m'}
+  (expr : CospanHyperGraph T n m) (expr' : CospanHyperGraph T n' m')
+  val val' :
+  Quote expr val -> Quote expr' val' ->
+  Quote (swapped_stack_graphs expr expr')
+    (swapped_stack_graphs val val').
+Proof.
+  apply (quote_of_binary_mor (fun _ => _) _).
+  intros; apply graph_apply_hom_swapped_stack_graphs.
+Qed.
+
+#[export] Instance cohg_quote_stack_graphs_aux {n m n' m'}
+  (expr : CospanHyperGraph T n m) (expr' : CospanHyperGraph T n' m')
+  val val' :
+  Quote expr val -> Quote expr' val' ->
+  Quote (stack_graphs_aux expr expr')
+    (stack_graphs_aux val val').
+Proof.
+  apply (quote_of_binary_mor (fun _ => _) _).
+  intros; apply graph_apply_hom_stack_graphs_aux.
+Qed.
+
+#[export] Instance cohg_quote_stack_graphs {n m n' m'}
+  (expr : CospanHyperGraph T n m) (expr' : CospanHyperGraph T n' m')
+  val val' :
+  Quote expr val -> Quote expr' val' ->
+  Quote (stack_graphs expr expr')
+    (stack_graphs val val').
+Proof.
+  apply (quote_of_binary_mor (fun _ => _) _).
+  intros; apply graph_apply_hom_stack_graphs.
+Qed.
+
+#[export] Instance cohg_quote_add_top_loop {n m}
+  (expr : CospanHyperGraph T (S n) (S m)) val :
+  Quote expr val ->
+  Quote (add_top_loop expr)
+    (add_top_loop val).
+Proof.
+  apply (quote_of_unary_mor (fun _ => _) _).
+  intros; apply graph_apply_hom_add_top_loop.
+Qed.
+
+#[export] Instance cohg_quote_add_top_loops {n m o}
+  (expr : CospanHyperGraph T (n + m) (n + o)) val :
+  Quote expr val ->
+  Quote (add_top_loops expr)
+    (add_top_loops val).
+Proof.
+  apply (quote_of_unary_mor (fun _ => _) _).
+  intros; apply graph_apply_hom_add_top_loops.
+Qed.
+
+#[export] Instance cohg_quote_compose_graphs_aux {n m o}
+  (expr : CospanHyperGraph T n m) (expr' : CospanHyperGraph T m o)
+  val val' :
+  Quote expr val -> Quote expr' val' ->
+  Quote (compose_graphs_aux expr expr')
+    (compose_graphs_aux val val').
+Proof.
+  apply (quote_of_binary_mor (fun _ => _) _).
+  intros; apply graph_apply_hom_compose_graphs_aux.
+Qed.
+
+#[export] Instance cohg_quote_compose_graphs {n m o}
+  (expr : CospanHyperGraph T n m) (expr' : CospanHyperGraph T m o)
+  val val' :
+  Quote expr val -> Quote expr' val' ->
+  Quote (compose_graphs expr expr')
+    (compose_graphs val val').
+Proof.
+  apply (quote_of_binary_mor (fun _ => _) _).
+  intros; apply graph_apply_hom_compose_graphs.
+Qed.
+
+#[export] Instance cohg_quote_compose_graphs_unsafe {n m o}
+  (expr : CospanHyperGraph T n m) (expr' : CospanHyperGraph T m o)
+  val val' :
+  Quote expr val -> Quote expr' val' ->
+  Quote (compose_graphs_unsafe expr expr')
+    (compose_graphs_unsafe val val').
+Proof.
+  apply (quote_of_binary_mor (fun _ => _) _).
+  intros; apply graph_apply_hom_compose_graphs_unsafe.
+Qed.
+
+#[export] Instance cohg_quote_norm_verts {n m}
+  (expr : CospanHyperGraph T n m) val :
+  Quote expr val ->
+  Quote (norm_verts expr)
+    (norm_verts val).
+Proof.
+  apply (quote_of_unary_mor (fun _ => _) _).
+  intros; apply graph_apply_hom_norm_verts.
+Qed.
+
+End instances.
+
+
+
+
+Class CospanHyperGraphDenote {Ctx T} `{Equiv T'} (f : Ctx -> T -> T')
+  (ctx : Ctx) {n m} (expr : CospanHyperGraph T n m) (val : CospanHyperGraph T' n m) := {
+  cohg_denote : cohg_eq (graph_apply_hom (f ctx) expr) val;
+}.
+
+#[global] Hint Mode CospanHyperGraphDenote + + + - + - + + + - : typeclass_instances.
+
+Class AbstractTensorDenote {Ctx T} `{Equiv T'} (f : Ctx -> T -> T') (ctx : Ctx)
+  (t : T) (t' : T') := {
+  abs_denote : f ctx t ≡ t'
+}.
+
+#[global] Hint Mode AbstractTensorDenote + + + - + + + - : typeclass_instances.
+
+#[export] Instance abstens_denote_default {Ctx T} `{Equiv T', Reflexive T' equiv}
+  (f : Ctx -> T -> T') (ctx : Ctx) (t : T) :
+  AbstractTensorDenote f ctx t (f ctx t) | 100.
+Proof.
+  constructor.
+  reflexivity.
+Qed.
+
+
+Lemma cohg_denote_correct_equiv {Ctx} `{Equiv T, Equivalence T equiv,
+  Equiv T', Equivalence T' equiv}
+  (f : Ctx -> T -> T')
+  (ctx : Ctx) {n m} (expr expr' : CospanHyperGraph T n m)
+    (val val' : CospanHyperGraph T' n m)
+    {Hval : CospanHyperGraphDenote f ctx expr val}
+    {Hval' : CospanHyperGraphDenote f ctx expr' val'}
+    {Hf : Proper (equiv ==> equiv) (f ctx)} :
+  expr ≡ expr' -> val ≡ val'.
+Proof.
+  intros Heq.
+  destruct Hval as [Hval].
+  destruct Hval' as [Hval'].
+  rewrite <- Hval.
+  etransitivity; [|apply cohg_eq_subrelation, Hval'].
+  refine (graph_apply_hom_proper_Proper _ _ _ _ _).
+  done.
+Qed.
+
+Section instances.
+
+#[local] Set Typeclasses Unique Instances.
+
+Context {Ctx T} `{Equiv T'} `{Equivalence T' equiv} (f : Ctx -> T -> T')
+  (ctx : Ctx).
+
+Local Notation Denote := (@CospanHyperGraphDenote Ctx T T' _ f ctx _ _).
+
+#[export] Instance cohg_denote_graph_apply_hom {n m} (expr : CospanHyperGraph T n m) :
+  Denote expr (graph_apply_hom (f ctx) expr).
+Proof.
+  now constructor.
+Qed.
+
+#[export] Instance cohg_denote_id_graph {n} : Denote (id_graph n) (id_graph n).
+Proof.
+  constructor.
+  done.
+Qed.
+
+#[export] Instance cohg_denote_cup_graph {n} : Denote (cup_graph n) (cup_graph n).
+Proof.
+  constructor.
+  done.
+Qed.
+
+#[export] Instance cohg_denote_cap_graph {n} : Denote (cap_graph n) (cap_graph n).
+Proof.
+  constructor.
+  done.
+Qed.
+
+#[export] Instance cohg_denote_swap_graph {n m} : Denote (swap_graph n m) (swap_graph n m).
+Proof.
+  constructor.
+  done.
+Qed.
+
+#[export] Instance cohg_denote_graph_of_tensor {n m} t t' :
+  AbstractTensorDenote f ctx t t' ->
+  Denote (graph_of_tensor t n m) (graph_of_tensor t' n m).
+Proof.
+  intros [Ht].
+  constructor.
+  rewrite graph_apply_hom_graph_of_tensor.
+  now apply graph_of_tensor_cohg_eq.
+Qed.
+
+Lemma denote_of_unary_mor {n m n' m'}
+  (g : forall T'', CospanHyperGraph T'' n m -> CospanHyperGraph T'' n' m')
+  (Hg : Proper (cohg_eq ==> cohg_eq) (g T'))
+  (Hghom : forall cohg, graph_apply_hom (f ctx) (g T cohg) =
+      g T' (graph_apply_hom (f ctx) cohg)) :
+  forall expr val, Denote expr val -> Denote (g T expr) (g T' val).
+Proof.
+  intros expr val [Hval].
+  constructor.
+  rewrite Hghom.
+  now apply Hg.
+Qed.
+
+Lemma denote_of_binary_mor {n m n' m' n'' m''}
+  (g : forall T'', CospanHyperGraph T'' n m -> CospanHyperGraph T'' n' m' ->
+    CospanHyperGraph T'' n'' m'')
+  (Hg : Proper (cohg_eq ==> cohg_eq ==> cohg_eq) (g T'))
+  (Hghom : forall cohg cohg', graph_apply_hom (f ctx) (g T cohg cohg') =
+      g T' (graph_apply_hom (f ctx) cohg) (graph_apply_hom (f ctx) cohg')) :
+  forall expr expr' val val', Denote expr val -> Denote expr' val' ->
+    Denote (g T expr expr') (g T' val val').
+Proof.
+  intros expr expr' val val' [Hval] [Hval'].
+  constructor.
+  rewrite Hghom.
+  now apply Hg.
+Qed.
+
+#[export] Instance cohg_denote_relabel_graph {n m}
+  g (expr : CospanHyperGraph T n m) val :
+  Denote expr val ->
+  Denote (relabel_graph g expr)
+    (relabel_graph g val).
+Proof.
+  apply (denote_of_unary_mor (fun _ => _) _).
+  intros; apply graph_apply_hom_relabel_graph.
+Qed.
+
+#[export] Instance cohg_denote_reindex_graph {n m}
+  g (expr : CospanHyperGraph T n m) val :
+  Denote expr val ->
+  Denote (reindex_graph g expr)
+    (reindex_graph g val).
+Proof.
+  apply (denote_of_unary_mor (fun _ => _) _).
+  intros; apply graph_apply_hom_reindex_graph.
+Qed.
+
+#[export] Instance cohg_denote_swapped_stack_graphs_aux {n m n' m'}
+  (expr : CospanHyperGraph T n m) (expr' : CospanHyperGraph T n' m')
+  val val' :
+  Denote expr val -> Denote expr' val' ->
+  Denote (swapped_stack_graphs_aux expr expr')
+    (swapped_stack_graphs_aux val val').
+Proof.
+  apply (denote_of_binary_mor (fun _ => _) _).
+  intros; apply graph_apply_hom_swapped_stack_graphs_aux.
+Qed.
+
+#[export] Instance cohg_denote_swapped_stack_graphs {n m n' m'}
+  (expr : CospanHyperGraph T n m) (expr' : CospanHyperGraph T n' m')
+  val val' :
+  Denote expr val -> Denote expr' val' ->
+  Denote (swapped_stack_graphs expr expr')
+    (swapped_stack_graphs val val').
+Proof.
+  apply (denote_of_binary_mor (fun _ => _) _).
+  intros; apply graph_apply_hom_swapped_stack_graphs.
+Qed.
+
+#[export] Instance cohg_denote_stack_graphs_aux {n m n' m'}
+  (expr : CospanHyperGraph T n m) (expr' : CospanHyperGraph T n' m')
+  val val' :
+  Denote expr val -> Denote expr' val' ->
+  Denote (stack_graphs_aux expr expr')
+    (stack_graphs_aux val val').
+Proof.
+  apply (denote_of_binary_mor (fun _ => _) _).
+  intros; apply graph_apply_hom_stack_graphs_aux.
+Qed.
+
+#[export] Instance cohg_denote_stack_graphs {n m n' m'}
+  (expr : CospanHyperGraph T n m) (expr' : CospanHyperGraph T n' m')
+  val val' :
+  Denote expr val -> Denote expr' val' ->
+  Denote (stack_graphs expr expr')
+    (stack_graphs val val').
+Proof.
+  apply (denote_of_binary_mor (fun _ => _) _).
+  intros; apply graph_apply_hom_stack_graphs.
+Qed.
+
+#[export] Instance cohg_denote_add_top_loop {n m}
+  (expr : CospanHyperGraph T (S n) (S m)) val :
+  Denote expr val ->
+  Denote (add_top_loop expr)
+    (add_top_loop val).
+Proof.
+  apply (denote_of_unary_mor (fun _ => _) _).
+  intros; apply graph_apply_hom_add_top_loop.
+Qed.
+
+#[export] Instance cohg_denote_add_top_loops {n m o}
+  (expr : CospanHyperGraph T (n + m) (n + o)) val :
+  Denote expr val ->
+  Denote (add_top_loops expr)
+    (add_top_loops val).
+Proof.
+  apply (denote_of_unary_mor (fun _ => _) _).
+  intros; apply graph_apply_hom_add_top_loops.
+Qed.
+
+#[export] Instance cohg_denote_compose_graphs_aux {n m o}
+  (expr : CospanHyperGraph T n m) (expr' : CospanHyperGraph T m o)
+  val val' :
+  Denote expr val -> Denote expr' val' ->
+  Denote (compose_graphs_aux expr expr')
+    (compose_graphs_aux val val').
+Proof.
+  apply (denote_of_binary_mor (fun _ => _) _).
+  intros; apply graph_apply_hom_compose_graphs_aux.
+Qed.
+
+#[export] Instance cohg_denote_compose_graphs {n m o}
+  (expr : CospanHyperGraph T n m) (expr' : CospanHyperGraph T m o)
+  val val' :
+  Denote expr val -> Denote expr' val' ->
+  Denote (compose_graphs expr expr')
+    (compose_graphs val val').
+Proof.
+  apply (denote_of_binary_mor (fun _ => _) _).
+  intros; apply graph_apply_hom_compose_graphs.
+Qed.
+
+#[export] Instance cohg_denote_compose_graphs_unsafe {n m o}
+  (expr : CospanHyperGraph T n m) (expr' : CospanHyperGraph T m o)
+  val val' :
+  Denote expr val -> Denote expr' val' ->
+  Denote (compose_graphs_unsafe expr expr')
+    (compose_graphs_unsafe val val').
+Proof.
+  apply (denote_of_binary_mor (fun _ => _) _).
+  intros; apply graph_apply_hom_compose_graphs_unsafe.
+Qed.
+
+#[export] Instance cohg_denote_norm_verts {n m}
+  (expr : CospanHyperGraph T n m) val :
+  Denote expr val ->
+  Denote (norm_verts expr)
+    (norm_verts val).
+Proof.
+  apply (denote_of_unary_mor (fun _ => _) _).
+  intros; apply graph_apply_hom_norm_verts.
+Qed.
+
+End instances.
+
+
+
+
+
+
+#[local] Program Instance opttensor_TensorLike
+  `{TensorLike R rO rI radd rmul req A T} : TensorLike R A (option T) := {
+  interpretTensor mt := from_option interpretTensor (fun _ _ => const_tensor rO) mt;
+}.
+Next Obligation.
+  intros *.
+  intros mt mt' Hmt.
+  induction Hmt as [mt mt' Hmt|]; [|done].
+  cbn.
+  now apply interpretTensorProper.
+Qed.
+
+#[export] Instance Some_TensorProper `{Equiv T} :
+  Proper (equiv ==> equiv) (@Some T) :=
+  Some_proper.
+
+#[export] Instance Some_TensorLikeHom `{TensorLike R rO rI radd rmul req A T} :
+  TensorLikeHom R A (@Some T).
+Proof.
+  split.
+  reflexivity.
+Qed.
+
+
+
+Lemma graph_to_option_correct_equiv
+  `{TensorLike R rO rI radd rmul req A T}
+  {n m} (expr expr' : CospanHyperGraph T n m) val val' :
+  CospanHyperGraphDenote (fun _ => Some) tt expr val ->
+  CospanHyperGraphDenote (fun _ => Some) tt expr' val' ->
+  val ≡ val' ->
+  expr ≡ expr'.
+Proof.
+  intros [Hval] [Hval'] Heq.
+  rewrite <- Hval, <- Hval' in Heq.
+  now apply (graph_apply_hom_equiv_inv Some).
+Qed.
+
+
+
+
+
+
+
+
+Inductive IsNth {A} : forall (a : A) (i : nat) (l : list A), Prop :=
+  | IsNth_here a l : IsNth a 0 (a :: l)
+  | IsNth_later a i a' l : IsNth a i l -> IsNth a (S i) (a' :: l).
+
+Lemma IsNth_iff_base {A} (a : A) i l :
+  IsNth a i l <-> (i < length l /\ forall d, nth i l d = a)%nat.
+Proof.
+  split.
+  - intros Hisn.
+    induction Hisn; (split; [cbn; lia|]).
+    + reflexivity.
+    + intros ?.
+      cbn.
+      easy.
+  - intros [Hil Hnth].
+    revert l Hil Hnth;
+    induction i; intros l Hil Hnth.
+    + destruct l; [easy|].
+      generalize (Hnth a).
+      cbn.
+      intros ->.
+      constructor.
+    + destruct l; [easy|].
+      cbn in Hil.
+      apply <- Nat.succ_lt_mono in Hil.
+      constructor.
+      auto.
+Qed.
+
+Lemma IsNth_iff {A} (a : A) i l :
+  IsNth a i l <-> l !! i = Some a.
+Proof.
+  split.
+  - intros Hisn.
+    induction Hisn; [done|].
+    cbn.
+    done.
+  - revert l;
+    induction i; intros l Hil.
+    + destruct l; [easy|].
+      cbn in Hil.
+      revert Hil.
+      intros [= ->].
+      constructor.
+    + destruct l; [easy|].
+      cbn in Hil.
+      constructor.
+      auto.
+Qed.
+
+
+
+(* On a goal [IsNth a ?i l], where [l] is [a0 :: a1 :: ... :: an :: ?l]
+  (i.e. ends in an evar), solves it with the smallest [i] such that
+  [a] and [ai] are convertible, or appends [a] to [l] if not (by
+  instantiating [?l := a :: ?l']). Assumes that [a] and all the [ai]
+  are ground terms (i.e. are not evars), and that [l] ends in an evar as
+  described above (if [a] is in [l], the latter condition is not necessary). *)
+Ltac get_nth :=
+  lazymatch goal with
+  | |- @IsNth ?A ?a ?i_evar ?l =>
+    tryif is_evar l then
+      idtac "evar" l;
+      let l' := fresh "l" in
+      evar (l' : list A);
+      let l' := eval unfold l' in l' in
+      refine (IsNth_here a l');
+      shelve
+    else
+      lazymatch l with
+      | ?a0 :: ?lrest =>
+        idtac "trying" a0;
+        tryif unify a a0 then
+          idtac "succeeded";
+          refine (IsNth_here a lrest);
+          shelve
+        else
+          idtac "failed";
+          refine (IsNth_later a _ a0 lrest _);
+          shelve_unifiable;
+          get_nth
+      | _ => fail "get_nth: list" l "is not an evar or a cons"
+      end
+  | |- ?G => fail "get_nth: goal is not of the form 'IsNth a ?i l' (goal:" G ")"
+  end.
+
+
+(* Splits a goal [Forall2 P l l'] according to the structure of [l].
+  In particular, if [l] is concrete and [l'] is an evar, [l'] will be
+  filled with evars to match the length of [l] *)
+Ltac split_forall2 := match goal with
+  | |- Forall2 _ (cons _ _) _ => apply List.Forall2_cons; [|split_forall2]
+  | |- Forall2 _ nil _ => apply List.Forall2_nil
+  | _ => idtac
+  end.
+
+(* To make the [IsNth] condition work, we use the following hint *)
+#[export] Hint Extern 0 (IsNth _ _ _) => get_nth : typeclass_instances.
+
+
+
+
+#[local] Instance positive_equiv : Equiv positive := eq.
+
+Definition interp_discrete_hg {T} (l : list T) (p : positive) :
+  option T :=
+  l !! (pos_to_nat_pred p).
+
+#[local] Instance interp_discrete_hg_proper `{Equiv T, Reflexive T equiv} ctx :
+  Proper (equiv ==> equiv) (@interp_discrete_hg T ctx).
+Proof.
+  intros ? ? [].
+  now apply option_Forall2_refl.
+Qed.
+
+#[export] Instance abstens_quote_discrete `{Equiv T, Reflexive T equiv}
+  (ctx : list T) (n : nat) (t : T) : IsNth t n ctx ->
+  AbstractTensorQuote interp_discrete_hg ctx (Pos.of_succ_nat n) (Some t).
+Proof.
+  intros Hn%IsNth_iff.
+  constructor.
+  unfold interp_discrete_hg.
+  rewrite pos_to_nat_pred_of_nat.
+  rewrite Hn.
+  now apply option_Forall2_refl.
+Qed.
+
+
+Lemma graph_equiv_of_positive `{Equiv T, Equivalence T equiv}
+  (ctx : list T) {n m} (expr expr' : CospanHyperGraph positive n m) val val' :
+  CospanHyperGraphQuote interp_discrete_hg ctx expr val ->
+  CospanHyperGraphQuote interp_discrete_hg ctx expr' val' ->
+  expr ≡ expr' ->
+  val ≡ val'.
+Proof.
+  intros Hval Hval'.
+  now apply (cohg_quote_correct_equiv interp_discrete_hg ctx), _.
+Qed.
+
+Lemma graph_test_isomorphism_quote `{Equiv T, Equivalence T equiv}
+  (ctx : list T) {n m} (expr expr' : CospanHyperGraph positive n m) val val' :
+  CospanHyperGraphQuote interp_discrete_hg ctx expr val ->
+  CospanHyperGraphQuote interp_discrete_hg ctx expr' val' ->
+  graph_iso_partial_test expr expr' = true ->
+  norm_verts val ≡ norm_verts val'.
+Proof.
+  intros Hval Hval' Heq%graph_iso_partial_test_correct.
+  revert Heq.
+  apply graph_equiv_of_positive with ctx; apply _.
+Qed.
+
+
+
+
